wip

src/QUIC.Impl.fst
@@ -79,8 +79,7 @@ let g_initial_packet_number #i s =
 let invariant_s #i h s =
   let open QUIC.Spec in
   let State hash_alg aead_alg traffic_secret initial_pn aead_state iv hp_key pn ctr_state =
-    s
-  in
+    s in
   hash_is_keysized s; (
   AEAD.invariant h aead_state /\
   not (B.g_is_null aead_state) /\
@@ -120,120 +119,14 @@ let packet_number_of_state #i s =
   let State _ _ _ _ _ _ _ pn _ = !*s in
   !*pn
 
-#push-options "--max_ifuel 1 --initial_ifuel 1"
-/// One ifuel for inverting on the hash algorithm for computing bounds (the
-/// various calls to assert_norm should help ensure this proof goes through
-/// reliably). Note that I'm breaking from the usual convention where lengths
-/// are UInt32's, mostly to avoid trouble reasoning with modulo when casting
-/// from UInt32 to UInt8 to write the label for the key derivation. This could
-/// be fixed later.
-val derive_secret: a: QUIC.Spec.ha ->
-  dst:B.buffer U8.t ->
-  dst_len: U8.t { B.length dst = U8.v dst_len /\ U8.v dst_len <= 255 } ->
-  secret:B.buffer U8.t { B.length secret = Spec.Hash.Definitions.hash_length a } ->
-  label:IB.ibuffer U8.t ->
-  label_len:U8.t { IB.length label = U8.v label_len /\ U8.v label_len <= 244 } ->
-  Stack unit
-    (requires fun h0 ->
-      B.(all_live h0 [ buf secret; buf label; buf dst ]) /\
-      B.disjoint dst secret)
-    (ensures fun h0 _ h1 ->
-      assert_norm (255 < pow2 61);
-      assert_norm (pow2 61 < pow2 125);
-      B.(modifies (loc_buffer dst) h0 h1) /\
-      B.as_seq h1 dst == QUIC.Spec.derive_secret a (B.as_seq h0 secret)
-        (IB.as_seq h0 label) (U8.v dst_len))
-#pop-options
+/// Helpers & globals
+/// -----------------
 
-let prefix = LowStar.ImmutableBuffer.igcmalloc_of_list HS.root QUIC.Spec.prefix_l
+friend QUIC.Impl.Lemmas
+open QUIC.Impl.Lemmas
 
-let lemma_five_cuts (s: S.seq U8.t) (i1 i2 i3 i4 i5: nat) (s0 s1 s2 s3 s4 s5: S.seq U8.t): Lemma
-  (requires (
-    i1 <= S.length s /\
-    i2 <= S.length s /\
-    i3 <= S.length s /\
-    i4 <= S.length s /\
-    i5 <= S.length s /\
-    i1 <= i2 /\
-    i2 <= i3 /\
-    i3 <= i4 /\
-    i4 <= i5 /\
-    s0 `Seq.equal` S.slice s 0 i1 /\
-    s1 `Seq.equal` S.slice s i1 i2 /\
-    s2 `Seq.equal` S.slice s i2 i3 /\
-    s3 `Seq.equal` S.slice s i3 i4 /\
-    s4 `Seq.equal` S.slice s i4 i5 /\
-    s5 `Seq.equal` S.slice s i5 (S.length s)))
-  (ensures (
-    let open S in
-    s `equal` (s0 @| s1 @| s2 @| s3 @| s4 @| s5)))
-=
-  ()
-
-let hash_is_keysized_ (a: QUIC.Spec.ha): Lemma
-  (ensures (QUIC.Spec.keysized a (Spec.Hash.Definitions.hash_length a)))
-=
-  assert_norm (512 < pow2 61);
-  assert_norm (512 < pow2 125)
-
-#set-options "--z3rlimit 100"
-let derive_secret a dst dst_len secret label label_len =
-  LowStar.ImmutableBuffer.recall prefix;
-  LowStar.ImmutableBuffer.recall_contents prefix QUIC.Spec.prefix;
-  (**) let h0 = ST.get () in
-
-  push_frame ();
-  (**) let h1 = ST.get () in
-
-  let label_len32 = FStar.Int.Cast.uint8_to_uint32 label_len in
-  let dst_len32 = FStar.Int.Cast.uint8_to_uint32 dst_len in
-  let info_len = U32.(1ul +^ 1ul +^ 1ul +^ 11ul +^ label_len32 +^ 1ul) in
-  let info = B.alloca 0uy info_len in
-
-  // JP: best way to reason about this sort of code is to slice the buffer very thinly
-  let info_z = B.sub info 0ul 1ul in
-  let info_lb = B.sub info 1ul 1ul in
-  let info_llen = B.sub info 2ul 1ul in
-  let info_prefix = B.sub info 3ul 11ul in
-  let info_label = B.sub info 14ul label_len32 in
-  let info_z' = B.sub info (14ul `U32.add` label_len32) 1ul in
-  (**) assert (14ul `U32.add` label_len32 `U32.add` 1ul = B.len info);
-  (**) assert B.(all_disjoint [ loc_buffer info_z; loc_buffer info_lb; loc_buffer info_llen;
-  (**)   loc_buffer info_prefix; loc_buffer info_label; loc_buffer info_z' ]);
-
-  info_lb.(0ul) <- dst_len;
-  info_llen.(0ul) <- U8.(label_len +^ 11uy);
-  B.blit prefix 0ul info_prefix 0ul 11ul;
-  B.blit label 0ul info_label 0ul label_len32;
-
-  (**) let h2 = ST.get () in
-  (**) assert (
-  (**)   let z = S.create 1 0uy in
-  (**)   let lb = S.create 1 dst_len in // len <= 255
-  (**)   let llen = S.create 1 (U8.uint_to_t (11 + Seq.length (B.as_seq h0 label))) in
-  (**)   let info = B.as_seq h2 info in
-  (**)   B.as_seq h2 info_z `Seq.equal` z /\
-  (**)   B.as_seq h2 info_lb `Seq.equal` lb /\
-  (**)   B.as_seq h2 info_llen `Seq.equal` llen /\
-  (**)   B.as_seq h2 info_prefix `Seq.equal` QUIC.Spec.prefix /\
-  (**)   B.as_seq h2 info_label `Seq.equal` (B.as_seq h0 label) /\
-  (**)   B.as_seq h2 info_z' `Seq.equal` z
-  (**) );
-  (**) (
-  (**)   let z = S.create 1 0uy in
-  (**)   let lb = S.create 1 dst_len in // len <= 255
-  (**)   let llen = S.create 1 (U8.uint_to_t (11 + Seq.length (B.as_seq h0 label))) in
-  (**)   let info = B.as_seq h2 info in
-  (**)   lemma_five_cuts info 1 2 3 14 (14 + U8.v label_len)
-  (**)     z lb llen QUIC.Spec.prefix (B.as_seq h0 label) z
-  (**) );
-  (**) hash_is_keysized_ a;
-  HKDF.expand a dst secret (Hacl.Hash.Definitions.hash_len a) info info_len dst_len32;
-  (**) let h3 = ST.get () in
-  pop_frame ();
-  (**) let h4 = ST.get () in
-  (**) B.modifies_fresh_frame_popped h0 h1 (B.loc_buffer dst) h3 h4;
-  (**) assert (ST.equal_domains h0 h4)
+inline_for_extraction noextract
+let u32_of_u8 = FStar.Int.Cast.uint8_to_uint32
 
 let key_len (a: QUIC.Spec.ea): x:U8.t { U8.v x = Spec.Agile.AEAD.key_length a } =
   let open Spec.Agile.AEAD in
@@ -247,273 +140,10 @@ let key_len32 a = FStar.Int.Cast.uint8_to_uint32 (key_len a)
 let label_key = LowStar.ImmutableBuffer.igcmalloc_of_list HS.root QUIC.Spec.label_key_l
 let label_iv = LowStar.ImmutableBuffer.igcmalloc_of_list HS.root QUIC.Spec.label_iv_l
 let label_hp = LowStar.ImmutableBuffer.igcmalloc_of_list HS.root QUIC.Spec.label_hp_l
+let prefix = LowStar.ImmutableBuffer.igcmalloc_of_list HS.root QUIC.Spec.prefix_l
 
-// JP: this proof currently takes 12 minutes. It could conceivably be improved.
-#push-options "--z3rlimit 1000 --query_stats"
-let create_in i r dst initial_pn traffic_secret =
-  LowStar.ImmutableBuffer.recall label_key;
-  LowStar.ImmutableBuffer.recall_contents label_key QUIC.Spec.label_key;
-  LowStar.ImmutableBuffer.recall label_iv;
-  LowStar.ImmutableBuffer.recall_contents label_iv QUIC.Spec.label_iv;
-  LowStar.ImmutableBuffer.recall label_hp;
-  LowStar.ImmutableBuffer.recall_contents label_hp QUIC.Spec.label_hp;
-  (**) let h0 = ST.get () in
-  [@inline_let]
-  let e_traffic_secret: G.erased (Spec.Hash.Definitions.bytes_hash i.hash_alg) =
-    G.hide (B.as_seq h0 traffic_secret)
-  in
-  [@inline_let]
-  let e_initial_pn: G.erased QUIC.Spec.nat62 = G.hide (U64.v initial_pn) in
-  [@inline_let]
-  let hash_alg = i.hash_alg in
-  [@inline_let]
-  let aead_alg = i.aead_alg in
-
-  push_frame ();
-  (**) let h1 = ST.get () in
-
-  let aead_key = B.alloca 0uy (key_len32 aead_alg) in
-  derive_secret hash_alg aead_key (key_len aead_alg) traffic_secret label_key 3uy;
-
-  (**) let h2 = ST.get () in
-  (**) B.(modifies_loc_includes (loc_unused_in h1) h1 h2 (loc_buffer aead_key));
-
-  let aead_state: B.pointer (B.pointer_or_null (AEAD.state_s aead_alg)) =
-    B.alloca B.null 1ul
-  in
-  let ret = AEAD.create_in #aead_alg r aead_state aead_key in
-
-  let ctr_state: B.pointer (B.pointer_or_null (CTR.state_s (as_cipher_alg aead_alg))) =
-    B.alloca (B.null #(CTR.state_s (as_cipher_alg aead_alg))) 1ul
-  in
-  let dummy_iv = B.alloca 0uy 12ul in
-  let ret' = CTR.create_in (as_cipher_alg aead_alg) r ctr_state aead_key dummy_iv 12ul 0ul in
-
-  (**) let h3 = ST.get () in
-  (**) B.(modifies_loc_includes (loc_unused_in h1) h2 h3
-    (loc_buffer ctr_state `loc_union` loc_buffer aead_state));
-  (**) B.(modifies_trans (loc_unused_in h1) h1 h2 (loc_unused_in h1) h3);
-
-  match ret with
-  | UnsupportedAlgorithm ->
-      pop_frame ();
-      UnsupportedAlgorithm
-
-  | Success ->
-
-      match ret' with
-      | UnsupportedAlgorithm ->
-          pop_frame ();
-          UnsupportedAlgorithm
-
-      | Success ->
-      // JP: there is something difficult to prove here... confused.
-      let aead_state: AEAD.state aead_alg = !*aead_state in
-      (**) assert (AEAD.invariant h3 aead_state);
-
-      let ctr_state: CTR.state (as_cipher_alg aead_alg) = !*ctr_state in
-      (**) assert (CTR.invariant h3 ctr_state);
-
-      let iv = B.malloc r 0uy 12ul in
-      (**) assert_norm FStar.Mul.(8 * 12 <= pow2 64 - 1);
-      (**) let h4 = ST.get () in
-      (**) B.(modifies_loc_includes (loc_buffer dst) h3 h4 loc_none);
-
-      let hp_key = B.malloc r 0uy (key_len32 aead_alg) in
-      (**) let h5 = ST.get () in
-      (**) B.(modifies_loc_includes (loc_buffer dst) h4 h5 loc_none);
-
-      let pn = B.malloc r initial_pn 1ul in
-      (**) let h6 = ST.get () in
-      (**) B.(modifies_loc_includes (loc_buffer dst) h5 h6 loc_none);
-
-      (**) assert (B.length hp_key = QUIC.Spec.ae_keysize aead_alg);
-      let s: state_s i = State #i
-        hash_alg aead_alg e_traffic_secret e_initial_pn
-        aead_state iv hp_key pn ctr_state
-      in
-      let s:B.pointer_or_null (state_s i) = B.malloc r s 1ul in
-      (**) let h7 = ST.get () in
-      (**) B.(modifies_loc_includes (loc_buffer dst) h6 h7 loc_none);
-
-      derive_secret hash_alg iv 12uy traffic_secret label_iv 2uy;
-      (**) let h8 = ST.get () in
-      (**) B.(modifies_loc_includes (loc_unused_in h1) h7 h8 (loc_buffer iv));
-
-      derive_secret hash_alg hp_key (key_len aead_alg) traffic_secret label_hp 2uy;
-      (**) let h9 = ST.get () in
-      (**) B.(modifies_loc_includes (loc_unused_in h1) h8 h9 (loc_buffer hp_key));
-      (**) B.(modifies_trans (loc_unused_in h1) h7 h8 (loc_unused_in h1) h9);
-
-      dst *= s;
-
-      (**) let h10 = ST.get () in
-      (**) B.(modifies_trans (loc_unused_in h1) h7 h9 (loc_buffer dst) h10);
-      (**) B.(modifies_trans (loc_unused_in h1) h1 h3 (loc_buffer dst) h7);
-      (**) B.(modifies_trans (loc_buffer dst) h3 h7
-      (**)   (loc_unused_in h1 `loc_union` loc_buffer dst) h10);
-      (**) B.(modifies_only_not_unused_in (loc_buffer dst) h1 h10);
-      (**) B.(modifies_only_not_unused_in (loc_buffer dst) h3 h10);
-      (**) B.fresh_frame_modifies h0 h1;
-      (**) B.(modifies_trans loc_none h0 h1 (loc_buffer dst) h10);
-
-      // TODO: everything goes through well up to here; and we know:
-      //   B.modifies (loc_buffer dst) h0 h10
-      // NOTE: how to conclude efficiently the same thing with h11?
-      pop_frame ();
-      (**) let h11 = ST.get () in
-      (**) assert (AEAD.invariant #aead_alg h11 aead_state);
-      (**) assert (CTR.invariant #(as_cipher_alg aead_alg) h11 ctr_state);
-      (**) B.popped_modifies h10 h11;
-      (**) assert B.(modifies (loc_buffer dst) h0 h11);
-      (**) assert (ST.equal_stack_domains h0 h11);
-
-      Success
-#pop-options
-
-let lemma_slice s (i: nat { i <= S.length s }): Lemma
-  (ensures (s `S.equal` S.append (S.slice s 0 i) (S.slice s i (S.length s))))
-=
-  ()
-
-#push-options "--max_fuel 1 --z3rlimit 100"
-let rec pointwise_upd (#a: eqtype) f b1 b2 i pos (x: a): Lemma
-  (requires (S.length b2 + pos <= S.length b1 /\ i < pos))
-  (ensures (S.upd (QUIC.Spec.pointwise_op f b1 b2 pos) i x `S.equal`
-    QUIC.Spec.pointwise_op f (S.upd b1 i x) b2 pos))
-  (decreases (S.length b2))
-=
-  calc (S.equal) {
-    QUIC.Spec.pointwise_op f (S.upd b1 i x) b2 pos;
-  (S.equal) { lemma_slice (S.upd b1 i x) (i + 1) }
-    QUIC.Spec.pointwise_op f
-      S.(slice (S.upd b1 i x) 0 (i + 1) @| S.slice (S.upd b1 i x) (i + 1) (S.length b1))
-      b2 pos;
-  (S.equal) { }
-    QUIC.Spec.pointwise_op f
-      S.(slice (S.upd b1 i x) 0 (i + 1) @| S.slice b1 (i + 1) (S.length b1))
-      b2 pos;
-  (S.equal) {
-    QUIC.Spec.pointwise_op_suff f
-      (S.slice (S.upd b1 i x) 0 (i + 1))
-      (S.slice b1 (i + 1) (S.length b1)) b2 pos
-  }
-    S.slice (S.upd b1 i x) 0 (i + 1) `S.append`
-    QUIC.Spec.pointwise_op f
-      (S.slice b1 (i + 1) (S.length b1))
-      b2 (pos - (i + 1));
-  (S.equal) { }
-    S.upd (S.slice b1 0 (i + 1)) i x `S.append`
-    QUIC.Spec.pointwise_op f
-      (S.slice b1 (i + 1) (S.length b1))
-      b2 (pos - (i + 1));
-  (S.equal) { }
-    S.upd (S.slice b1 0 (i + 1) `S.append`
-    QUIC.Spec.pointwise_op f
-      (S.slice b1 (i + 1) (S.length b1))
-      b2 (pos - (i + 1))
-    ) i x;
-  (S.equal) {
-    QUIC.Spec.pointwise_op_suff f
-      (S.slice b1 0 (i + 1))
-      (S.slice b1 (i + 1) (S.length b1)) b2 pos
-  }
-    S.upd (
-      QUIC.Spec.pointwise_op f
-      (S.slice b1 0 (i + 1) `S.append` S.slice b1 (i + 1) (S.length b1))
-      b2 pos
-    ) i x;
-  (S.equal) { lemma_slice b1 (i + 1) }
-    S.upd (QUIC.Spec.pointwise_op f b1 b2 pos) i x;
-  }
-
-let rec pointwise_seq_map2 (#a: eqtype) (f: a -> a -> a) (s1 s2: S.seq a) (i: nat): Lemma
-  (requires (
-    let l = S.length s1 in
-    S.length s2 = l - i /\ i <= S.length s1))
-  (ensures (
-    let l = S.length s1 in
-    Spec.Loops.seq_map2 f (S.slice s1 i l) s2 `S.equal`
-    S.slice (QUIC.Spec.pointwise_op f s1 s2 i) i l))
-  (decreases (S.length s2))
-=
-  if S.length s2 = 0 then
-    ()
-  else
-    let l = S.length s1 in
-    calc (S.equal) {
-      Spec.Loops.seq_map2 f (S.slice s1 i l) s2;
-    (S.equal) {}
-      S.cons (f (S.head (S.slice s1 i l)) (S.head s2))
-        (Spec.Loops.seq_map2 f (S.tail (S.slice s1 i l)) (S.tail s2));
-    (S.equal) {}
-      S.cons (f (S.head (S.slice s1 i l)) (S.head s2))
-        (Spec.Loops.seq_map2 f (S.slice s1 (i + 1) l) (S.tail s2));
-    (S.equal) { pointwise_seq_map2 f s1 (S.slice s2 1 (S.length s2)) (i + 1) }
-      S.cons (f (S.head (S.slice s1 i l)) (S.head s2))
-        (S.slice (QUIC.Spec.pointwise_op f s1 (S.tail s2) (i + 1)) (i + 1) l);
-    (S.equal) { }
-      S.slice (
-        S.upd (QUIC.Spec.pointwise_op f s1 (S.tail s2) (i + 1))
-          i
-          (f (S.head (S.slice s1 i l)) (S.head s2)))
-        i
-        l;
-    (S.equal) { }
-      S.slice (
-        S.upd (QUIC.Spec.pointwise_op f s1 (S.slice s2 1 (S.length s2)) (i + 1))
-          i
-          (f (S.head (S.slice s1 i l)) (S.head s2)))
-        i
-        l;
-    (S.equal) {
-      pointwise_upd f s1 (S.slice s2 1 (S.length s2)) i (i + 1)
-        (f (S.head (S.slice s1 i l)) (S.head s2))
-    }
-      S.slice
-        (QUIC.Spec.pointwise_op f
-          (S.upd s1 i (f (S.head (S.slice s1 i l)) (S.head s2)))
-          (S.slice s2 1 (S.length s2))
-          (i + 1))
-        i l;
-
-    };
-    ()
-#pop-options
-
-#push-options "--max_fuel 2 --initial_fuel 2 --max_ifuel 1 --initial_ifuel 1"
-let rec and_inplace_commutative (s1 s2: S.seq U8.t): Lemma
-  (requires S.length s1 = S.length s2)
-  (ensures Spec.Loops.seq_map2 U8.logand s1 s2 `S.equal`
-    Spec.Loops.seq_map2 U8.logand s2 s1)
-  (decreases (S.length s1))
-=
-  if S.length s1 = 0 then
-    ()
-  else (
-    FStar.UInt.logand_commutative #8 (U8.v (S.head s1)) (U8.v (S.head s2));
-    assert (U8.logand (S.head s1) (S.head s2) = U8.logand (S.head s2) (S.head s1));
-    and_inplace_commutative (S.tail s1) (S.tail s2);
-    assert (Spec.Loops.seq_map2 U8.logand (S.tail s1) (S.tail s2) `S.equal`
-      Spec.Loops.seq_map2 U8.logand (S.tail s2) (S.tail s1))
-  )
-#pop-options
-
-let lemma_slice3 #a (s: S.seq a) (i j: nat): Lemma
-  (requires (i <= j /\ j <= S.length s))
-  (ensures (s `S.equal`
-    (S.slice s 0 i `S.append` S.slice s i j `S.append` S.slice s j (S.length s))))
-=
-  ()
-
-let lemma_slice0 #a (s: S.seq a): Lemma (S.slice s 0 (S.length s) `S.equal` s) = ()
-
-let lemma_slice1 #a (s: S.seq a) (i j: nat): Lemma
-  (requires (i <= j /\ j <= S.length s))
-  (ensures (S.slice s 0 j `S.equal`
-    (S.slice s 0 i `S.append` S.slice s i j)))
-=
-  ()
+/// Actual code
+/// -----------
 
 #push-options "--z3rlimit 200"
 inline_for_extraction noextract
@@ -596,6 +226,267 @@ let op_inplace (dst: B.buffer U8.t)
       (B.as_seq h0 src)
       (U32.v ofs);
   }
+
+#push-options "--max_ifuel 1 --initial_ifuel 1"
+/// One ifuel for inverting on the hash algorithm for computing bounds (the
+/// various calls to assert_norm should help ensure this proof goes through
+/// reliably). Note that I'm breaking from the usual convention where lengths
+/// are UInt32's, mostly to avoid trouble reasoning with modulo when casting
+/// from UInt32 to UInt8 to write the label for the key derivation. This could
+/// be fixed later.
+val derive_secret: a: QUIC.Spec.ha ->
+  dst:B.buffer U8.t ->
+  dst_len: U8.t { B.length dst = U8.v dst_len /\ U8.v dst_len <= 255 } ->
+  secret:B.buffer U8.t { B.length secret = Spec.Hash.Definitions.hash_length a } ->
+  label:IB.ibuffer U8.t ->
+  label_len:U8.t { IB.length label = U8.v label_len /\ U8.v label_len <= 244 } ->
+  Stack unit
+    (requires fun h0 ->
+      B.(all_live h0 [ buf secret; buf label; buf dst ]) /\
+      B.disjoint dst secret)
+    (ensures fun h0 _ h1 ->
+      assert_norm (255 < pow2 61);
+      assert_norm (pow2 61 < pow2 125);
+      B.(modifies (loc_buffer dst) h0 h1) /\
+      B.as_seq h1 dst == QUIC.Spec.derive_secret a (B.as_seq h0 secret)
+        (IB.as_seq h0 label) (U8.v dst_len))
+#pop-options
+
+#push-options "--z3rlimit 100"
+let derive_secret a dst dst_len secret label label_len =
+  LowStar.ImmutableBuffer.recall prefix;
+  LowStar.ImmutableBuffer.recall_contents prefix QUIC.Spec.prefix;
+  (**) let h0 = ST.get () in
+
+  push_frame ();
+  (**) let h1 = ST.get () in
+
+  let label_len32 = FStar.Int.Cast.uint8_to_uint32 label_len in
+  let dst_len32 = FStar.Int.Cast.uint8_to_uint32 dst_len in
+  let info_len = U32.(1ul +^ 1ul +^ 1ul +^ 11ul +^ label_len32 +^ 1ul) in
+  let info = B.alloca 0uy info_len in
+
+  // JP: best way to reason about this sort of code is to slice the buffer very thinly
+  let info_z = B.sub info 0ul 1ul in
+  let info_lb = B.sub info 1ul 1ul in
+  let info_llen = B.sub info 2ul 1ul in
+  let info_prefix = B.sub info 3ul 11ul in
+  let info_label = B.sub info 14ul label_len32 in
+  let info_z' = B.sub info (14ul `U32.add` label_len32) 1ul in
+  (**) assert (14ul `U32.add` label_len32 `U32.add` 1ul = B.len info);
+  (**) assert B.(all_disjoint [ loc_buffer info_z; loc_buffer info_lb; loc_buffer info_llen;
+  (**)   loc_buffer info_prefix; loc_buffer info_label; loc_buffer info_z' ]);
+
+  info_lb.(0ul) <- dst_len;
+  info_llen.(0ul) <- U8.(label_len +^ 11uy);
+  B.blit prefix 0ul info_prefix 0ul 11ul;
+  B.blit label 0ul info_label 0ul label_len32;
+
+  (**) let h2 = ST.get () in
+  (**) assert (
+  (**)   let z = S.create 1 0uy in
+  (**)   let lb = S.create 1 dst_len in // len <= 255
+  (**)   let llen = S.create 1 (U8.uint_to_t (11 + Seq.length (B.as_seq h0 label))) in
+  (**)   let info = B.as_seq h2 info in
+  (**)   B.as_seq h2 info_z `Seq.equal` z /\
+  (**)   B.as_seq h2 info_lb `Seq.equal` lb /\
+  (**)   B.as_seq h2 info_llen `Seq.equal` llen /\
+  (**)   B.as_seq h2 info_prefix `Seq.equal` QUIC.Spec.prefix /\
+  (**)   B.as_seq h2 info_label `Seq.equal` (B.as_seq h0 label) /\
+  (**)   B.as_seq h2 info_z' `Seq.equal` z
+  (**) );
+  (**) (
+  (**)   let z = S.create 1 0uy in
+  (**)   let lb = S.create 1 dst_len in // len <= 255
+  (**)   let llen = S.create 1 (U8.uint_to_t (11 + Seq.length (B.as_seq h0 label))) in
+  (**)   let info = B.as_seq h2 info in
+  (**)   lemma_five_cuts info 1 2 3 14 (14 + U8.v label_len)
+  (**)     z lb llen QUIC.Spec.prefix (B.as_seq h0 label) z
+  (**) );
+  (**) hash_is_keysized_ a;
+  HKDF.expand a dst secret (Hacl.Hash.Definitions.hash_len a) info info_len dst_len32;
+  (**) let h3 = ST.get () in
+  pop_frame ();
+  (**) let h4 = ST.get () in
+  (**) B.modifies_fresh_frame_popped h0 h1 (B.loc_buffer dst) h3 h4;
+  (**) assert (ST.equal_domains h0 h4)
+#pop-options
+
+val create_in_core:
+  i:index ->
+  r:HS.rid ->
+  dst: B.pointer (B.pointer_or_null (state_s i)) ->
+  initial_pn:u62 ->
+  traffic_secret:B.buffer U8.t {
+    B.length traffic_secret = Spec.Hash.Definitions.hash_length i.hash_alg
+  } ->
+  aead_state:AEAD.state i.aead_alg ->
+  ctr_state:CTR.state (as_cipher_alg i.aead_alg) ->
+  ST unit
+    (requires fun h0 ->
+      QUIC.Impl.Lemmas.hash_is_keysized_ i.hash_alg; (
+      ST.is_eternal_region r /\
+      B.live h0 dst /\ B.live h0 traffic_secret /\
+      B.(all_disjoint [ AEAD.footprint h0 aead_state; CTR.footprint h0 ctr_state;
+        loc_buffer dst; loc_buffer traffic_secret ]) /\
+      B.(loc_includes (loc_region_only true r) (AEAD.footprint h0 aead_state)) /\
+      B.(loc_includes (loc_region_only true r) (CTR.footprint h0 ctr_state)) /\
+
+      // Whatever from the invariant ought to be established already.
+      AEAD.invariant h0 aead_state /\
+      not (B.g_is_null aead_state) /\
+      CTR.invariant h0 ctr_state /\
+      not (B.g_is_null ctr_state) /\
+      AEAD.as_kv (B.deref h0 aead_state) ==
+        QUIC.Spec.(derive_secret i.hash_alg (B.as_seq h0 traffic_secret) label_key
+          (Spec.Agile.AEAD.key_length i.aead_alg))))
+    (ensures (fun h0 _ h1 ->
+      let s = B.deref h1 dst in
+      not (B.g_is_null s) /\
+      invariant h1 s /\
+
+      B.(modifies (loc_buffer dst) h0 h1) /\ (
+      let State _ _ _ initial_pn' aead_state' iv' hp_key' pn' ctr_state' = B.deref h1 s in
+      aead_state' == aead_state /\
+      ctr_state' == ctr_state /\
+      B.(fresh_loc (loc_buffer iv') h0 h1) /\
+      B.(fresh_loc (loc_buffer hp_key') h0 h1) /\
+      B.(fresh_loc (loc_buffer pn') h0 h1) /\
+      B.(fresh_loc (loc_addr_of_buffer s) h0 h1) /\
+
+      G.reveal initial_pn' == U64.v initial_pn)))
+
+#push-options "--z3rlimit 50"
+let create_in_core i r dst initial_pn traffic_secret aead_state ctr_state =
+  LowStar.ImmutableBuffer.recall label_key;
+  LowStar.ImmutableBuffer.recall_contents label_key QUIC.Spec.label_key;
+  LowStar.ImmutableBuffer.recall label_iv;
+  LowStar.ImmutableBuffer.recall_contents label_iv QUIC.Spec.label_iv;
+  LowStar.ImmutableBuffer.recall label_hp;
+  LowStar.ImmutableBuffer.recall_contents label_hp QUIC.Spec.label_hp;
+
+  (**) let h0 = ST.get () in
+  (**) assert_norm FStar.Mul.(8 * 12 <= pow2 64 - 1);
+  let mloc = G.hide (B.(loc_buffer dst `loc_union` loc_unused_in h0)) in
+  let e_traffic_secret: G.erased (Spec.Hash.Definitions.bytes_hash i.hash_alg) =
+    G.hide (B.as_seq h0 traffic_secret) in
+  let e_initial_pn: G.erased QUIC.Spec.nat62 = G.hide (U64.v initial_pn) in
+
+  let iv = B.malloc r 0uy 12ul in
+  let hp_key = B.malloc r 0uy (key_len32 i.aead_alg) in
+  let pn = B.malloc r initial_pn 1ul in
+  (**) let h1 = ST.get () in
+  (**) B.(modifies_loc_includes (G.reveal mloc) h0 h1 loc_none);
+  (**) assert (B.length hp_key = QUIC.Spec.ae_keysize i.aead_alg);
+
+  let s: state_s i = State #i
+    i.hash_alg i.aead_alg e_traffic_secret e_initial_pn
+    aead_state iv hp_key pn ctr_state
+  in
+
+  let s:B.pointer_or_null (state_s i) = B.malloc r s 1ul in
+  (**) let h2 = ST.get () in
+  (**) B.(modifies_loc_includes (G.reveal mloc) h1 h2 loc_none);
+  (**) B.(modifies_trans (G.reveal mloc) h0 h1 (G.reveal mloc) h2);
+
+  derive_secret i.hash_alg iv 12uy traffic_secret label_iv 2uy;
+  (**) let h3 = ST.get () in
+  (**) B.(modifies_loc_includes (G.reveal mloc) h2 h3 (loc_buffer iv));
+  (**) B.(modifies_trans (G.reveal mloc) h0 h2 (G.reveal mloc) h3);
+
+  derive_secret i.hash_alg hp_key (key_len i.aead_alg) traffic_secret label_hp 2uy;
+  (**) let h4 = ST.get () in
+  (**) B.(modifies_loc_includes (G.reveal mloc) h3 h4 (loc_buffer hp_key));
+  (**) B.(modifies_trans (G.reveal mloc) h0 h3 (G.reveal mloc) h4);
+
+  dst *= s;
+  (**) let h5 = ST.get () in
+  (**) B.(modifies_loc_includes (G.reveal mloc) h4 h5 (loc_buffer dst));
+  (**) B.(modifies_trans (G.reveal mloc) h0 h4 (G.reveal mloc) h5);
+  (**) B.(modifies_only_not_unused_in (loc_buffer dst) h0 h5)
+#pop-options
+
+#push-options "--z3rlimit 200"
+let create_in i r dst initial_pn traffic_secret =
+  LowStar.ImmutableBuffer.recall label_key;
+  LowStar.ImmutableBuffer.recall_contents label_key QUIC.Spec.label_key;
+
+  (**) let h0 = ST.get () in
+
+  push_frame ();
+  (**) let h1 = ST.get () in
+  let mloc = G.hide (B.(loc_region_only true (HS.get_tip h1) `loc_union` loc_buffer dst
+    `loc_union` loc_unused_in h0)) in
+
+  let aead_key = B.alloca 0uy (key_len32 i.aead_alg) in
+  let aead_state: B.pointer (B.pointer_or_null (AEAD.state_s i.aead_alg)) =
+    B.alloca B.null 1ul in
+  let ctr_state: B.pointer (B.pointer_or_null (CTR.state_s (as_cipher_alg i.aead_alg))) =
+    B.alloca (B.null #(CTR.state_s (as_cipher_alg i.aead_alg))) 1ul in
+  let dummy_iv = B.alloca 0uy 12ul in
+
+  (**) let h2 = ST.get () in
+  (**) B.(modifies_loc_includes (G.reveal mloc) h1 h2 (loc_none));
+
+  derive_secret i.hash_alg aead_key (key_len i.aead_alg) traffic_secret label_key 3uy;
+  (**) let h3 = ST.get () in
+  (**) B.(modifies_loc_includes (G.reveal mloc) h2 h3 (loc_buffer aead_key));
+  (**) B.(modifies_trans (G.reveal mloc) h1 h2 (G.reveal mloc) h3);
+
+  let ret = AEAD.create_in #i.aead_alg r aead_state aead_key in
+  (**) let h4 = ST.get () in
+  (**) B.(modifies_loc_includes (G.reveal mloc) h3 h4 (loc_buffer aead_state));
+  (**) B.(modifies_trans (G.reveal mloc) h1 h3 (G.reveal mloc) h4);
+
+  let ret' = CTR.create_in (as_cipher_alg i.aead_alg) r ctr_state aead_key dummy_iv 12ul 0ul in
+  (**) let h5 = ST.get () in
+  (**) B.(modifies_loc_includes (G.reveal mloc) h4 h5 (loc_buffer ctr_state));
+  (**) B.(modifies_trans (G.reveal mloc) h1 h4 (G.reveal mloc) h5);
+  (**) B.(modifies_only_not_unused_in B.(loc_region_only true (HS.get_tip h1) `loc_union` loc_buffer dst) h1 h5);
+
+  match ret with
+  | UnsupportedAlgorithm ->
+      pop_frame ();
+      (**) let h6 = ST.get () in
+      (**) B.(modifies_fresh_frame_popped h0 h1 (loc_buffer dst) h5 h6);
+      UnsupportedAlgorithm
+
+  | Success ->
+
+  match ret' with
+  | UnsupportedAlgorithm ->
+      pop_frame ();
+      (**) let h6 = ST.get () in
+      (**) B.(modifies_fresh_frame_popped h0 h1 (loc_buffer dst) h5 h6);
+      UnsupportedAlgorithm
+
+  | Success ->
+
+      let aead_state: AEAD.state i.aead_alg = !*aead_state in
+      (**) assert (AEAD.invariant h5 aead_state);
+
+      let ctr_state: CTR.state (as_cipher_alg i.aead_alg) = !*ctr_state in
+      (**) assert (CTR.invariant h5 ctr_state);
+
+      create_in_core i r dst initial_pn traffic_secret aead_state ctr_state;
+      (**) let h6 = ST.get () in
+
+      (**) B.(modifies_loc_includes
+        (loc_region_only true (HS.get_tip h1) `loc_union` loc_buffer dst) h5 h6
+        (loc_buffer dst));
+      (**) B.(modifies_trans
+        (loc_region_only true (HS.get_tip h1) `loc_union` loc_buffer dst)
+        h1 h5
+        (loc_region_only true (HS.get_tip h1) `loc_union` loc_buffer dst)
+        h6);
+
+      pop_frame ();
+      (**) let h7 = ST.get () in
+      (**) B.(modifies_fresh_frame_popped h0 h1 (loc_buffer dst) h6 h7);
+      admit ();
+
+      Success
+#pop-options
 
 
 let format_header (dst: B.buffer U8.t) (h: header) (npn: B.buffer U8.t) (pn_len: u2):
@@ -812,7 +703,7 @@ val header_encrypt: i:G.erased index -> (
         QUIC.Spec.header_encrypt i.aead_alg (g_hp_key h0 s) (g_header h h0)
           (B.as_seq h0 npn) (G.reveal cipher) /\
       invariant h1 s /\
-      footprint h0 s == footprint h1 s))
+      footprint_s h0 (B.deref h0 s) == footprint_s h1 (B.deref h1 s)))
 
 #push-options "--max_fuel 2 --initial_fuel 2 --max_ifuel 1 --initial_ifuel 1"
 let upd_op_inplace (#a:eqtype) op (s: S.seq a) (x: a): Lemma
@@ -915,74 +806,6 @@ let header_encrypt i dst dst_len s h cipher iv npn pn_len =
   (**) let h7 = ST.get () in
   ()
 
-open FStar.Mul
-
-let rec be_to_n_slice (s: S.seq U8.t) (i: nat): Lemma
-  (requires i <= S.length s)
-  (ensures FStar.Endianness.be_to_n (S.slice s i (S.length s)) =
-    FStar.Endianness.be_to_n s % pow2 (8 `op_Multiply` (S.length s - i)))
-  (decreases (S.length s))
-=
-  FStar.Endianness.reveal_be_to_n s;
-  if S.length s = 0 then
-    ()
-  else
-    let open FStar.Endianness in
-    if i = S.length s then begin
-      reveal_be_to_n S.empty;
-      assert_norm (pow2 (8 * 0) = 1);
-      assert (S.slice s (S.length s) (S.length s) `S.equal` S.empty);
-      assert (be_to_n S.empty = 0);
-      assert (be_to_n s % 1 = 0)
-    end else
-      let s' = (S.slice s i (S.length s)) in
-      let s_prefix = (S.slice s 0 (S.length s - 1)) in
-      assert (S.length s' <> 0);
-      assert (8 <= 8 * (S.length s - i));
-      FStar.Math.Lemmas.pow2_le_compat (8 * (S.length s - i)) 8;
-      assert_norm (pow2 (8 * 1) = 256);
-      assert (U8.v (S.last s) < pow2 (8 * (S.length s - i)));
-      assert (S.length s' = S.length s_prefix - i + 1);
-      FStar.Math.Lemmas.pow2_le_compat (8 * (S.length s')) (8 * (S.length s - i));
-      calc (==) {
-        be_to_n s';
-      (==) {
-        lemma_be_to_n_is_bounded s';
-        FStar.Math.Lemmas.small_mod (be_to_n s') (pow2 (8 * (S.length s - i)))
-      }
-        (be_to_n s') % (pow2 (8 * (S.length s - i)));
-      (==) { reveal_be_to_n s' }
-        (U8.v (S.last s') + pow2 8 * be_to_n (S.slice s' 0 (S.length s' - 1))) %
-          (pow2 (8 * (S.length s - i)));
-      (==) { }
-        (U8.v (S.last s) + pow2 8 * be_to_n (S.slice s i (S.length s - 1))) %
-          (pow2 (8 * (S.length s - i)));
-      (==) { }
-        (U8.v (S.last s) + pow2 8 * (be_to_n (S.slice s_prefix i (S.length s_prefix)))) %
-          (pow2 (8 * (S.length s - i)));
-      (==) { be_to_n_slice s_prefix i }
-        (U8.v (S.last s) + pow2 8 * (be_to_n s_prefix % pow2 (8 * (S.length s_prefix - i)))) %
-          (pow2 (8 * (S.length s - i)));
-      (==) { FStar.Math.Lemmas.pow2_multiplication_modulo_lemma_2
-        (be_to_n s_prefix) (8 * (S.length s_prefix - i) + 8) 8
-      }
-        (U8.v (S.last s) +
-          ((be_to_n s_prefix * pow2 8) % pow2 (8 * (S.length s_prefix - i) + 8))
-        ) %
-          (pow2 (8 * (S.length s - i)));
-      (==) { }
-        (U8.v (S.last s) +
-          ((be_to_n s_prefix * pow2 8) % pow2 (8 * (S.length s - i)))
-        ) %
-          (pow2 (8 * (S.length s - i)));
-      (==) { FStar.Math.Lemmas.lemma_mod_add_distr
-        (U8.v (S.last s))
-        (be_to_n s_prefix * pow2 8)
-        (pow2 (8 * (S.length s - i)))
-      }
-        (U8.v (S.last s) + pow2 8 * be_to_n (S.slice s 0 (S.length s - 1))) %
-          pow2 (8 * (S.length s - i));
-      }
 
 let tag_len (a: QUIC.Spec.ea): x:U32.t { U32.v x = Spec.Agile.AEAD.tag_length a /\ U32.v x = 16} =
   let open Spec.Agile.AEAD in
@@ -1005,147 +828,208 @@ let tricky_addition (aead_alg: QUIC.Spec.ea) (h: header) (pn_len: u2) (plain_len
 =
   header_len h pn_len `U32.add` plain_len `U32.add` tag_len aead_alg
 
-#set-options "--query_stats --z3rlimit 1000"
-let encrypt #i s dst h plain plain_len pn_len =
-  // [@inline_let]
-  let u32_of_u8 = FStar.Int.Cast.uint8_to_uint32 in
+open FStar.Mul
+
+val encrypt_core: #i:G.erased index -> (
+  let i = G.reveal i in
+  s:state i ->
+  dst:B.buffer U8.t ->
+  h:header ->
+  plain: B.buffer U8.t ->
+  plain_len: U32.t {
+    3 <= U32.v plain_len /\
+    U32.v plain_len < QUIC.Spec.max_plain_length /\
+    B.length plain = U32.v plain_len
+  } ->
+  pn_len: u2 ->
+  stack: G.erased B.loc ->
+  pnb:B.buffer U8.t ->
+  this_iv:B.buffer U8.t ->
+  Stack unit
+    (requires fun h0 ->
+      assert_norm (pow2 62 < pow2 (8 * 12));
+      let stack = G.reveal stack in
+      // Memory & preservation
+      B.(all_live h0 [ buf dst; buf plain; buf pnb; buf this_iv ]) /\
+      header_live h h0 /\
+      header_disjoint h /\
+      B.(all_disjoint [ stack; footprint h0 s; loc_buffer dst;
+        header_footprint h; loc_buffer plain ]) /\
+
+      invariant h0 s /\
+
+      // Local stuff
+      B.(loc_includes stack (loc_buffer pnb)) /\
+      B.(loc_includes stack (loc_buffer this_iv)) /\
+      B.(disjoint pnb this_iv) /\
+      B.length pnb = 12 /\
+      B.length this_iv = 12 /\
+      B.as_seq h0 pnb `S.equal`
+        FStar.Endianness.n_to_be 12 (g_packet_number (B.deref h0 s) h0) /\
+
+      incrementable s h0 /\ (
+      let clen = U32.v plain_len + Spec.Agile.AEAD.tag_length i.aead_alg in
+      let len = clen + QUIC.Spec.header_len (g_header h h0) (U8.v pn_len) in
+      (Long? h ==> U32.v (Long?.plain_len h) = clen) /\
+      B.length dst == len
+    ))
+    (ensures fun h0 r h1 ->
+        // Memory & preservation
+        B.(modifies (stack `loc_union`
+          footprint_s h0 (deref h0 s) `loc_union` loc_buffer dst)) h0 h1 /\
+        invariant h1 s /\
+        footprint_s h1 (B.deref h1 s) == footprint_s h0 (B.deref h0 s) /\ (
+
+        // Functional correctness
+        let s0 = g_traffic_secret (B.deref h0 s) in
+        let open QUIC.Spec in
+        let k = derive_secret i.hash_alg s0 label_key (Spec.Agile.AEAD.key_length i.aead_alg) in
+        let iv = derive_secret i.hash_alg s0 label_iv 12 in
+        let pne = derive_secret i.hash_alg s0 label_hp (ae_keysize i.aead_alg) in
+        let plain: pbytes = B.as_seq h0 plain in
+        let packet: packet = B.as_seq h1 dst in
+        let ctr = g_packet_number (B.deref h0 s) h0 in
+        packet ==
+          QUIC.Spec.encrypt i.aead_alg k iv pne (U8.v pn_len) ctr (g_header h h0) plain)))
+
+let encrypt_core #i s dst h plain plain_len pn_len stack pnb this_iv =
+  (**) let h0 = ST.get () in
+  (**) let m_loc = G.hide B.(G.reveal stack `loc_union`
+  (**)   footprint_s h0 (deref h0 s) `loc_union` loc_buffer dst) in
+  (**) assert_norm (pow2 62 < pow2 (8 * 12));
+
   let State hash_alg aead_alg e_traffic_secret e_initial_pn
     aead_state iv hp_key pn ctr_state = !*s
   in
-  (**) let h0 = ST.get () in
-  (**) assert (
-  (**)   let s0 = g_traffic_secret (B.deref h0 s) in
-  (**)   let open QUIC.Spec in
-  (**)   let k = derive_secret i.hash_alg s0 label_key (Spec.Agile.AEAD.key_length i.aead_alg) in
-  (**)   let iv_seq = derive_secret i.hash_alg s0 label_iv 12 in
-  (**)   let hp_key_seq = derive_secret i.hash_alg s0 label_hp (ae_keysize i.aead_alg) in
-  (**)   AEAD.as_kv (B.deref h0 aead_state) `S.equal` k /\
-  (**)   B.as_seq h0 iv `S.equal` iv_seq /\
-  (**)   B.as_seq h0 hp_key `S.equal` hp_key_seq);
-
-  push_frame ();
-  (**) let h01 = ST.get () in
-  let pnb0 = B.alloca 0uy 16ul in
-  (**) assert B.(loc_includes (loc_all_regions_from false (HS.get_tip h01)) (loc_buffer pnb0));
-  (**) B.(modifies_loc_includes
-    (loc_all_regions_from false (HS.get_tip h01) `loc_union`
-      footprint_s h0 (deref h0 s) `loc_union` loc_buffer dst)
-    h0 h01 (loc_all_regions_from false (HS.get_tip h01)));
-
-  // JP: cannot inline this in the call below; why?
-  let pn: U64.t = !*pn in
-  let pn128: FStar.UInt128.t = FStar.Int.Cast.Full.uint64_to_uint128 pn in
-  LowStar.Endianness.store128_be pnb0 pn128;
-  (**) let h02 = ST.get () in
-  (**) frame_invariant B.(loc_buffer pnb0) s h01 h02;
-  (**) B.(modifies_loc_includes
-    (loc_all_regions_from false (HS.get_tip h01) `loc_union`
-      footprint_s h0 (deref h0 s) `loc_union` loc_buffer dst)
-    h01 h02 (loc_all_regions_from false (HS.get_tip h01)));
-
-  let pnb = B.sub pnb0 4ul 12ul in
-  (**) let h1 = ST.get () in
-  (**) (
-  (**) let open FStar.Endianness in
-  (**) assert_norm (pow2 64 < pow2 (8 * 12));
-  (**) calc (==) {
-  (**)   be_to_n (B.as_seq h1 pnb);
-  (**) (==) { }
-  (**)   be_to_n (S.slice (B.as_seq h1 pnb0) 4 16);
-  (**) (==) { be_to_n_slice (B.as_seq h1 pnb0) 4 }
-  (**)   be_to_n (B.as_seq h1 pnb0) % pow2 (8 * 12);
-  (**) (==) { FStar.Math.Lemmas.small_mod (U64.v pn) (pow2 (8 * 12)) }
-  (**)   be_to_n (B.as_seq h1 pnb0);
-  (**) });
-  (**) assert (B.as_seq h1 pnb `S.equal`
-  (**)   FStar.Endianness.n_to_be 12 (g_packet_number (B.deref h1 s) h1));
-
   let npn = B.sub pnb (11ul `U32.sub` u32_of_u8 pn_len) (1ul `U32.add` u32_of_u8 pn_len) in
-  (**) assert (B.as_seq h1 npn `S.equal` S.slice (B.as_seq h1 pnb) (11 - U8.v pn_len) 12);
   let dst_h = B.sub dst 0ul (header_len h pn_len) in
   let dst_ciphertag = B.sub dst (header_len h pn_len) (plain_len `U32.add` tag_len aead_alg) in
   let dst_cipher = B.sub dst_ciphertag 0ul plain_len in
   let dst_tag = B.sub dst_ciphertag plain_len (tag_len aead_alg) in
+
   format_header dst_h h npn pn_len;
-  (**) let h10 = ST.get () in
-  (**) frame_invariant B.(loc_buffer dst) s h02 h10;
-  (**) assert (let h_len = QUIC.Spec.header_len (g_header h h0) (U8.v pn_len) in
-  (**)   S.slice (B.as_seq h10 dst) 0 h_len `S.equal`
-  (**)     QUIC.Spec.format_header (g_header h h10) (B.as_seq h10 npn));
-  (**) assert B.(loc_includes (loc_buffer dst) (loc_buffer dst_h));
-  (**) B.(modifies_loc_includes
-    (loc_all_regions_from false (HS.get_tip h01) `loc_union`
-      footprint_s h0 (deref h0 s) `loc_union` loc_buffer dst)
-    h1 h10 (loc_buffer dst));
-
-
+  (**) let h1 = ST.get () in
+  (**) frame_invariant B.(loc_buffer dst) s h0 h1;
+  (**) assert (footprint_s h0 (B.deref h0 s) == footprint_s h1 (B.deref h1 s));
+  (**) B.(modifies_loc_includes (G.reveal m_loc) h0 h1 (loc_buffer dst));
   (**) QUIC.Spec.lemma_format_len aead_alg (g_header h h0) (B.as_seq h1 npn);
-  let this_iv = B.alloca 0uy 12ul in
-  (**) let h11 = ST.get () in
-  (**) assert B.(loc_includes (loc_all_regions_from false (HS.get_tip h01)) (loc_buffer this_iv));
-  (**) B.(modifies_loc_includes
-    (loc_all_regions_from false (HS.get_tip h01) `loc_union`
-      footprint_s h0 (deref h0 s) `loc_union` loc_buffer dst)
-    h10 h11 (loc_all_regions_from false (HS.get_tip h01)));
 
   C.Loops.map2 this_iv pnb iv 12ul U8.logxor;
-  (**) pointwise_seq_map2 U8.logxor (B.as_seq h10 pnb) (B.as_seq h10 iv) 0;
   (**) let h2 = ST.get () in
-  (**) assert (let h_len = QUIC.Spec.header_len (g_header h h0) (U8.v pn_len) in
-  (**)   S.slice (B.as_seq h2 dst) 0 h_len `S.equal`
-  (**)     QUIC.Spec.format_header (g_header h h2) (B.as_seq h2 npn));
-  (**) frame_invariant B.(loc_buffer this_iv) s h10 h2;
-  // JP: hard
-  (**) assert (footprint_s h0 (B.deref h0 s) == footprint_s h2 (B.deref h2 s));
-  (**) B.(modifies_loc_includes
-    (loc_all_regions_from false (HS.get_tip h01) `loc_union`
-      footprint_s h0 (deref h0 s) `loc_union` loc_buffer dst)
-    h11 h2 (loc_all_regions_from false (HS.get_tip h01)));
+  (**) frame_invariant B.(loc_buffer this_iv) s h1 h2;
+  (**) assert (footprint_s h1 (B.deref h1 s) == footprint_s h2 (B.deref h2 s));
+  (**) B.(modifies_loc_includes (G.reveal m_loc) h1 h2 (loc_buffer this_iv));
+  (**) B.(modifies_trans (G.reveal m_loc) h0 h1 (G.reveal m_loc) h2);
+  (**) pointwise_seq_map2 U8.logxor (B.as_seq h1 pnb) (B.as_seq h1 iv) 0;
+  (**) assert (
+    let open QUIC.Spec in
+    let npn: lbytes (1 + U8.v pn_len) = S.slice (B.as_seq h0 pnb) (11 - U8.v pn_len) 12 in
+    let s0 = g_traffic_secret (B.deref h0 s) in
+    let siv = derive_secret i.hash_alg s0 label_iv 12 in
+    B.as_seq h2 this_iv `S.equal` xor_inplace (B.as_seq h0 pnb) siv 0
+  );
 
   let l = header_len h pn_len in
-  // JP: adding assert here SIGNIFICANTLY reduces verification time; what's hard?
-  (**) assert (AEAD.encrypt_pre aead_alg aead_state this_iv 12ul dst_h l
-  (**)   plain plain_len dst_cipher dst_tag h2);
   let r = AEAD.encrypt #(G.hide aead_alg) aead_state
     this_iv 12ul dst_h (header_len h pn_len) plain plain_len dst_cipher dst_tag in
-  (**) assert (r = Success);
   (**) let h3 = ST.get () in
-  // JP: incredibly hard; takes two minutes extra on my machine to prove this
-  (**) assert (footprint_s h2 (B.deref h2 s) == footprint_s h3 (B.deref h3 s));
   (**) assert (invariant h3 s);
-  // JP: also hard
-  (**) assert B.(modifies (AEAD.footprint h2 aead_state `loc_union` loc_buffer dst_cipher
-  (**)   `loc_union` loc_buffer dst_tag) h2 h3);
-  (**) assert B.(loc_includes (footprint_s h2 (B.deref h2 s)) (AEAD.footprint h2 aead_state));
-  (**) assert B.(loc_includes (loc_buffer dst)
-  (**)   (loc_buffer dst_cipher `loc_union` loc_buffer dst_tag));
-  // JP: adds a minute
-  B.(modifies_loc_includes
-    (loc_all_regions_from false (HS.get_tip h01) `loc_union`
-      footprint_s h0 (deref h0 s) `loc_union` loc_buffer dst)
-    h2 h3 (footprint_s h0 (deref h0 s) `loc_union` loc_buffer dst));
+  (**) assert (footprint_s h2 (B.deref h2 s) == footprint_s h2 (B.deref h3 s));
+  (**) B.(modifies_loc_includes (G.reveal m_loc) h2 h3
+    (AEAD.footprint h2 aead_state `loc_union` loc_buffer dst));
+  (**) B.(modifies_trans (G.reveal m_loc) h0 h2 (G.reveal m_loc) h3);
+  (**) assert (r = Success);
+  (**) assert (
+    let open QUIC.Spec in
+    let s0 = g_traffic_secret (B.deref h0 s) in
+    let siv = derive_secret i.hash_alg s0 label_iv 12 in
+    let k = derive_secret i.hash_alg s0 label_key (Spec.Agile.AEAD.key_length i.aead_alg) in
+    let seqn = g_packet_number (B.deref h0 s) h0 in
+    let h = g_header h h0 in
+    let plain = B.as_seq h0 plain in
+    let a = aead_alg in
 
-  // JP: without this side definition, this is an extra 30s of verification time
+    let pnb = FStar.Endianness.n_to_be 12 seqn  in
+    let npn: lbytes (1 + U8.v pn_len) = S.slice pnb (11 - U8.v pn_len) 12 in
+    let header = format_header h npn in
+    let iv = xor_inplace pnb siv 0 in
+    let cipher = Spec.Agile.AEAD.encrypt #a k iv header plain in
+    cipher `S.equal` B.as_seq h3 dst_ciphertag
+  );
+
   let dst_len = tricky_addition aead_alg h pn_len plain_len in
-  (**) assert (B.length dst = U32.v dst_len);
-  (**) assert (B.length dst_ciphertag >= 19);
-  (**) assert (B.length dst_ciphertag < QUIC.Spec.max_cipher_length);
-  (**) let e_cipher:G.erased (QUIC.Spec.cbytes) = G.elift1
-  (**)   (fun (b: B.buffer U8.t { B.length b = B.length dst_ciphertag }) ->
-  (**)     ((B.as_seq h3 b) <: QUIC.Spec.cbytes)) (G.hide dst_ciphertag)
-  (**) in
-  (**) let e_iv = G.elift1 (B.as_seq h2) (G.hide pnb) in
-  (**) assert (let h_len = QUIC.Spec.header_len (g_header h h0) (U8.v pn_len) in
-  (**)   S.slice (B.as_seq h3 dst) 0 h_len `S.equal`
-  (**)     QUIC.Spec.format_header (g_header h h3) (B.as_seq h3 npn));
-  (**) assert (header_encrypt_pre (G.reveal i) dst dst_len s h e_cipher e_iv npn pn_len h3);
+  let e_cipher = G.hide ((B.as_seq h3 dst_ciphertag) <: QUIC.Spec.cbytes) in
+  let e_iv = G.hide (B.as_seq h3 this_iv) in
   header_encrypt i dst dst_len s h e_cipher e_iv npn pn_len;
   (**) let h4 = ST.get () in
-  (**) B.(modifies_loc_includes
-    (loc_all_regions_from false (HS.get_tip h01) `loc_union`
-      footprint_s h0 (deref h0 s) `loc_union` loc_buffer dst)
-    h3 h4 (footprint_s h0 (deref h0 s) `loc_union` loc_buffer dst));
   (**) assert (invariant h4 s);
+  (**) assert (footprint_s h3 (B.deref h3 s) == footprint_s h4 (B.deref h4 s));
+  (**) B.(modifies_loc_includes (G.reveal m_loc) h3 h4
+    (footprint_s h3 (B.deref h3 s) `loc_union` loc_buffer dst));
+  (**) B.(modifies_trans (G.reveal m_loc) h0 h3 (G.reveal m_loc) h4);
+  (**) assert (
+    let open QUIC.Spec in
+    let s0 = g_traffic_secret (B.deref h0 s) in
+    let siv = derive_secret i.hash_alg s0 label_iv 12 in
+    let k = derive_secret i.hash_alg s0 label_key (Spec.Agile.AEAD.key_length i.aead_alg) in
+    let seqn = g_packet_number (B.deref h0 s) h0 in
+    let h = g_header h h0 in
+    let plain = B.as_seq h0 plain in
+    let a = aead_alg in
+    let hpk = g_hp_key h0 s in
+    let pn_len = U8.v pn_len in
+
+    B.as_seq h4 dst `S.equal` QUIC.Spec.encrypt a k siv hpk pn_len seqn h plain
+  )
+
+#set-options "--query_stats --z3rlimit 1000"
+let encrypt #i s dst h plain plain_len pn_len =
+  (**) let h0 = ST.get () in
+  let State hash_alg aead_alg e_traffic_secret e_initial_pn
+    aead_state iv hp_key pn ctr_state = !*s
+  in
+
+  push_frame ();
+  (**) let h1 = ST.get () in
+  (**) let mloc = G.hide B.(loc_all_regions_from false (HS.get_tip h1) `loc_union`
+    footprint_s h0 (deref h0 s) `loc_union` loc_buffer dst) in
+
+  let pnb0 = B.alloca 0uy 16ul in
+  let this_iv = B.alloca 0uy 12ul in
+  (**) let h2 = ST.get () in
+  (**) frame_invariant B.(loc_none) s h1 h2;
+  (**) assert (footprint_s h1 (B.deref h1 s) == footprint_s h2 (B.deref h2 s));
+  (**) B.(modifies_loc_includes (G.reveal mloc) h1 h2 loc_none);
+
+  let pn: U64.t = !*pn in
+  let pn128: FStar.UInt128.t = FStar.Int.Cast.Full.uint64_to_uint128 pn in
+  LowStar.Endianness.store128_be pnb0 pn128;
+  (**) let h3 = ST.get () in
+  (**) frame_invariant B.(loc_buffer pnb0) s h2 h3;
+  (**) assert (footprint_s h2 (B.deref h2 s) == footprint_s h3 (B.deref h3 s));
+  (**) B.(modifies_trans (G.reveal mloc) h1 h2 (G.reveal mloc) h3);
+
+  let pnb = B.sub pnb0 4ul 12ul in
+  (**) (
+  (**) let open FStar.Endianness in
+  (**) assert_norm (pow2 64 < pow2 (8 * 12));
+  (**) calc (==) {
+  (**)   be_to_n (B.as_seq h3 pnb);
+  (**) (==) { }
+  (**)   be_to_n (S.slice (B.as_seq h3 pnb0) 4 16);
+  (**) (==) { be_to_n_slice (B.as_seq h3 pnb0) 4 }
+  (**)   be_to_n (B.as_seq h3 pnb0) % pow2 (8 * 12);
+  (**) (==) { FStar.Math.Lemmas.small_mod (U64.v pn) (pow2 (8 * 12)) }
+  (**)   be_to_n (B.as_seq h3 pnb0);
+  (**) });
+  (**) assert (B.as_seq h3 pnb `S.equal`
+  (**)   FStar.Endianness.n_to_be 12 (g_packet_number (B.deref h0 s) h0));
+
+  (**) assert B.(loc_disjoint (loc_region_only true (B.frameOf s))
+  (**)   (loc_all_regions_from false (HS.get_tip h1)));
+  encrypt_core #i s dst h plain plain_len pn_len
+    (G.hide B.(loc_all_regions_from false (HS.get_tip h1))) pnb this_iv;
+
   pop_frame ();
 
   (**) let h5 = ST.get () in
@@ -1167,11 +1051,12 @@ let encrypt #i s dst h plain plain_len pn_len =
   (**)   B.(modifies (footprint_s h0 (deref h0 s) `loc_union` loc_buffer dst)) h0 h5);
   (**) assert B.(modifies (loc_all_regions_from false (HS.get_tip h01) `loc_union`
   (**)   footprint_s h0 (deref h0 s) `loc_union` loc_buffer dst) h01 h4);
+  (**) assert (footprint_s h4 (B.deref h4 s) == footprint_s h3 (B.deref h3 s));
 
   (**) B.popped_modifies h4 h5;
   (**) frame_invariant B.(loc_region_only false (HS.get_tip h4)) s h4 h5;
   (**) assert (invariant h5 s);
-  (**) assert (footprint h4 s == footprint h3 s);
+  (**) assert (footprint_s h0 (B.deref h0 s) == footprint_s h3 (B.deref h3 s));
 
   admit ();
 
