src/QUIC.Impl.Lemmas.fst
@@ -1,0 +1,265 @@
+module QUIC.Impl.Lemmas
+
+module G = FStar.Ghost
+module S = FStar.Seq
+
+module U64 = FStar.UInt64
+module U32 = FStar.UInt32
+module U8 = FStar.UInt8
+
+friend QUIC.Spec
+
+#set-options "--max_fuel 0 --max_ifuel 0"
+
+/// The usual sequence lemmas
+/// -------------------------
+
+let lemma_five_cuts (s: S.seq U8.t) (i1 i2 i3 i4 i5: nat) (s0 s1 s2 s3 s4 s5: S.seq U8.t): Lemma
+  (requires (
+    i1 <= S.length s /\
+    i2 <= S.length s /\
+    i3 <= S.length s /\
+    i4 <= S.length s /\
+    i5 <= S.length s /\
+    i1 <= i2 /\
+    i2 <= i3 /\
+    i3 <= i4 /\
+    i4 <= i5 /\
+    s0 `Seq.equal` S.slice s 0 i1 /\
+    s1 `Seq.equal` S.slice s i1 i2 /\
+    s2 `Seq.equal` S.slice s i2 i3 /\
+    s3 `Seq.equal` S.slice s i3 i4 /\
+    s4 `Seq.equal` S.slice s i4 i5 /\
+    s5 `Seq.equal` S.slice s i5 (S.length s)))
+  (ensures (
+    let open S in
+    s `equal` (s0 @| s1 @| s2 @| s3 @| s4 @| s5)))
+=
+  ()
+
+let hash_is_keysized_ (a: QUIC.Spec.ha): Lemma
+  (ensures (QUIC.Spec.keysized a (Spec.Hash.Definitions.hash_length a)))
+=
+  assert_norm (512 < pow2 61);
+  assert_norm (512 < pow2 125)
+
+
+let lemma_slice s (i: nat { i <= S.length s }): Lemma
+  (ensures (s `S.equal` S.append (S.slice s 0 i) (S.slice s i (S.length s))))
+=
+  ()
+
+let lemma_slice3 #a (s: S.seq a) (i j: nat): Lemma
+  (requires (i <= j /\ j <= S.length s))
+  (ensures (s `S.equal`
+    (S.slice s 0 i `S.append` S.slice s i j `S.append` S.slice s j (S.length s))))
+=
+  ()
+
+let lemma_slice0 #a (s: S.seq a): Lemma (S.slice s 0 (S.length s) `S.equal` s) = ()
+
+let lemma_slice1 #a (s: S.seq a) (i j: nat): Lemma
+  (requires (i <= j /\ j <= S.length s))
+  (ensures (S.slice s 0 j `S.equal`
+    (S.slice s 0 i `S.append` S.slice s i j)))
+=
+  ()
+
+
+open FStar.Mul
+
+/// Lemmas about pointwise_op (needs friending)
+/// -------------------------------------------
+
+#push-options "--max_fuel 1 --z3rlimit 100"
+let rec pointwise_upd (#a: eqtype) f b1 b2 i pos (x: a): Lemma
+  (requires (S.length b2 + pos <= S.length b1 /\ i < pos))
+  (ensures (S.upd (QUIC.Spec.pointwise_op f b1 b2 pos) i x `S.equal`
+    QUIC.Spec.pointwise_op f (S.upd b1 i x) b2 pos))
+  (decreases (S.length b2))
+=
+  calc (S.equal) {
+    QUIC.Spec.pointwise_op f (S.upd b1 i x) b2 pos;
+  (S.equal) { lemma_slice (S.upd b1 i x) (i + 1) }
+    QUIC.Spec.pointwise_op f
+      S.(slice (S.upd b1 i x) 0 (i + 1) @| S.slice (S.upd b1 i x) (i + 1) (S.length b1))
+      b2 pos;
+  (S.equal) { }
+    QUIC.Spec.pointwise_op f
+      S.(slice (S.upd b1 i x) 0 (i + 1) @| S.slice b1 (i + 1) (S.length b1))
+      b2 pos;
+  (S.equal) {
+    QUIC.Spec.pointwise_op_suff f
+      (S.slice (S.upd b1 i x) 0 (i + 1))
+      (S.slice b1 (i + 1) (S.length b1)) b2 pos
+  }
+    S.slice (S.upd b1 i x) 0 (i + 1) `S.append`
+    QUIC.Spec.pointwise_op f
+      (S.slice b1 (i + 1) (S.length b1))
+      b2 (pos - (i + 1));
+  (S.equal) { }
+    S.upd (S.slice b1 0 (i + 1)) i x `S.append`
+    QUIC.Spec.pointwise_op f
+      (S.slice b1 (i + 1) (S.length b1))
+      b2 (pos - (i + 1));
+  (S.equal) { }
+    S.upd (S.slice b1 0 (i + 1) `S.append`
+    QUIC.Spec.pointwise_op f
+      (S.slice b1 (i + 1) (S.length b1))
+      b2 (pos - (i + 1))
+    ) i x;
+  (S.equal) {
+    QUIC.Spec.pointwise_op_suff f
+      (S.slice b1 0 (i + 1))
+      (S.slice b1 (i + 1) (S.length b1)) b2 pos
+  }
+    S.upd (
+      QUIC.Spec.pointwise_op f
+      (S.slice b1 0 (i + 1) `S.append` S.slice b1 (i + 1) (S.length b1))
+      b2 pos
+    ) i x;
+  (S.equal) { lemma_slice b1 (i + 1) }
+    S.upd (QUIC.Spec.pointwise_op f b1 b2 pos) i x;
+  }
+
+let rec pointwise_seq_map2 (#a: eqtype) (f: a -> a -> a) (s1 s2: S.seq a) (i: nat): Lemma
+  (requires (
+    let l = S.length s1 in
+    S.length s2 = l - i /\ i <= S.length s1))
+  (ensures (
+    let l = S.length s1 in
+    Spec.Loops.seq_map2 f (S.slice s1 i l) s2 `S.equal`
+    S.slice (QUIC.Spec.pointwise_op f s1 s2 i) i l))
+  (decreases (S.length s2))
+=
+  if S.length s2 = 0 then
+    ()
+  else
+    let l = S.length s1 in
+    calc (S.equal) {
+      Spec.Loops.seq_map2 f (S.slice s1 i l) s2;
+    (S.equal) {}
+      S.cons (f (S.head (S.slice s1 i l)) (S.head s2))
+        (Spec.Loops.seq_map2 f (S.tail (S.slice s1 i l)) (S.tail s2));
+    (S.equal) {}
+      S.cons (f (S.head (S.slice s1 i l)) (S.head s2))
+        (Spec.Loops.seq_map2 f (S.slice s1 (i + 1) l) (S.tail s2));
+    (S.equal) { pointwise_seq_map2 f s1 (S.slice s2 1 (S.length s2)) (i + 1) }
+      S.cons (f (S.head (S.slice s1 i l)) (S.head s2))
+        (S.slice (QUIC.Spec.pointwise_op f s1 (S.tail s2) (i + 1)) (i + 1) l);
+    (S.equal) { }
+      S.slice (
+        S.upd (QUIC.Spec.pointwise_op f s1 (S.tail s2) (i + 1))
+          i
+          (f (S.head (S.slice s1 i l)) (S.head s2)))
+        i
+        l;
+    (S.equal) { }
+      S.slice (
+        S.upd (QUIC.Spec.pointwise_op f s1 (S.slice s2 1 (S.length s2)) (i + 1))
+          i
+          (f (S.head (S.slice s1 i l)) (S.head s2)))
+        i
+        l;
+    (S.equal) {
+      pointwise_upd f s1 (S.slice s2 1 (S.length s2)) i (i + 1)
+        (f (S.head (S.slice s1 i l)) (S.head s2))
+    }
+      S.slice
+        (QUIC.Spec.pointwise_op f
+          (S.upd s1 i (f (S.head (S.slice s1 i l)) (S.head s2)))
+          (S.slice s2 1 (S.length s2))
+          (i + 1))
+        i l;
+
+    };
+    ()
+#pop-options
+
+#push-options "--max_fuel 2 --initial_fuel 2 --max_ifuel 1 --initial_ifuel 1"
+let rec and_inplace_commutative (s1 s2: S.seq U8.t): Lemma
+  (requires S.length s1 = S.length s2)
+  (ensures Spec.Loops.seq_map2 U8.logand s1 s2 `S.equal`
+    Spec.Loops.seq_map2 U8.logand s2 s1)
+  (decreases (S.length s1))
+=
+  if S.length s1 = 0 then
+    ()
+  else (
+    FStar.UInt.logand_commutative #8 (U8.v (S.head s1)) (U8.v (S.head s2));
+    assert (U8.logand (S.head s1) (S.head s2) = U8.logand (S.head s2) (S.head s1));
+    and_inplace_commutative (S.tail s1) (S.tail s2);
+    assert (Spec.Loops.seq_map2 U8.logand (S.tail s1) (S.tail s2) `S.equal`
+      Spec.Loops.seq_map2 U8.logand (S.tail s2) (S.tail s1))
+  )
+#pop-options
+
+/// Endianness lemmas
+/// -----------------
+
+let rec be_to_n_slice (s: S.seq U8.t) (i: nat): Lemma
+  (requires i <= S.length s)
+  (ensures FStar.Endianness.be_to_n (S.slice s i (S.length s)) =
+    FStar.Endianness.be_to_n s % pow2 (8 `op_Multiply` (S.length s - i)))
+  (decreases (S.length s))
+=
+  FStar.Endianness.reveal_be_to_n s;
+  if S.length s = 0 then
+    ()
+  else
+    let open FStar.Endianness in
+    if i = S.length s then begin
+      reveal_be_to_n S.empty;
+      assert_norm (pow2 (8 * 0) = 1);
+      assert (S.slice s (S.length s) (S.length s) `S.equal` S.empty);
+      assert (be_to_n S.empty = 0);
+      assert (be_to_n s % 1 = 0)
+    end else
+      let s' = (S.slice s i (S.length s)) in
+      let s_prefix = (S.slice s 0 (S.length s - 1)) in
+      assert (S.length s' <> 0);
+      assert (8 <= 8 * (S.length s - i));
+      FStar.Math.Lemmas.pow2_le_compat (8 * (S.length s - i)) 8;
+      assert_norm (pow2 (8 * 1) = 256);
+      assert (U8.v (S.last s) < pow2 (8 * (S.length s - i)));
+      assert (S.length s' = S.length s_prefix - i + 1);
+      FStar.Math.Lemmas.pow2_le_compat (8 * (S.length s')) (8 * (S.length s - i));
+      calc (==) {
+        be_to_n s';
+      (==) {
+        lemma_be_to_n_is_bounded s';
+        FStar.Math.Lemmas.small_mod (be_to_n s') (pow2 (8 * (S.length s - i)))
+      }
+        (be_to_n s') % (pow2 (8 * (S.length s - i)));
+      (==) { reveal_be_to_n s' }
+        (U8.v (S.last s') + pow2 8 * be_to_n (S.slice s' 0 (S.length s' - 1))) %
+          (pow2 (8 * (S.length s - i)));
+      (==) { }
+        (U8.v (S.last s) + pow2 8 * be_to_n (S.slice s i (S.length s - 1))) %
+          (pow2 (8 * (S.length s - i)));
+      (==) { }
+        (U8.v (S.last s) + pow2 8 * (be_to_n (S.slice s_prefix i (S.length s_prefix)))) %
+          (pow2 (8 * (S.length s - i)));
+      (==) { be_to_n_slice s_prefix i }
+        (U8.v (S.last s) + pow2 8 * (be_to_n s_prefix % pow2 (8 * (S.length s_prefix - i)))) %
+          (pow2 (8 * (S.length s - i)));
+      (==) { FStar.Math.Lemmas.pow2_multiplication_modulo_lemma_2
+        (be_to_n s_prefix) (8 * (S.length s_prefix - i) + 8) 8
+      }
+        (U8.v (S.last s) +
+          ((be_to_n s_prefix * pow2 8) % pow2 (8 * (S.length s_prefix - i) + 8))
+        ) %
+          (pow2 (8 * (S.length s - i)));
+      (==) { }
+        (U8.v (S.last s) +
+          ((be_to_n s_prefix * pow2 8) % pow2 (8 * (S.length s - i)))
+        ) %
+          (pow2 (8 * (S.length s - i)));
+      (==) { FStar.Math.Lemmas.lemma_mod_add_distr
+        (U8.v (S.last s))
+        (be_to_n s_prefix * pow2 8)
+        (pow2 (8 * (S.length s - i)))
+      }
+        (U8.v (S.last s) + pow2 8 * be_to_n (S.slice s 0 (S.length s - 1))) %
+          pow2 (8 * (S.length s - i));
+      }
